\documentclass{article}
\usepackage{xcolor}
\usepackage{tikz}
\usepackage{parskip}
\usepackage{amsmath}
\usepackage{amsthm}
\usepackage{amssymb}
\usepackage{mathtools}
\usepackage{fancyhdr}
\usepackage[%paperheight = 59.4cm,
            %paperwidth = 42cm,
            %includehead,
            nomarginpar,
            textwidth=15cm,
            headheight=10mm]{geometry}


\begin{document}

\pagestyle{fancy}
%\fancyhead{}\fancyfoot{}

\fancyhf[OHC]{Christopher Munoz WRH6 Diffeq}
\setcounter{section}{4}
\setcounter{subsection}{4}
\setcounter{subsubsection}{1}
\subsubsection{}
a) We are provided the second order differential equation $ y'' - 9y' = 3x^2 - 5\sin(3x) $ and we are tasked with finding the form of the particular solution, by first inspection/observation we find the form to be:
\begin{align}
    \Aboxed{y_p &= (Ax^2 + Bx + C) + D\cos(3x) + E\sin(3x)}
\end{align}
b) We are also provided with the second order differential equation $ y'' + 2y' + y = 2e^{-x} - e^x$, by inspection/observation we conclude that the form of the particular solution is:
\begin{align*}
    \Aboxed{y_p = Ae^{-x} + Be^x}
\end{align*}
\subsubsection{} 
We are tasked with solving the following differential equations via method of undetermined coefficients: \\ \\ a) $ y'' + 2y' = 2x + 5 - e^{-2x} $ \\
\setcounter{equation}{0}
\begin{align*}
    & y'' + 2y' = 2x + 5 - e^{-2x} &  y_p = Ax^2 + Bx + Cxe^{-2x} \\
    & m^2 + 2m + 0 = 0 & y_p' = 2Ax +B - 2Cxe^{-2x} + Ce^{-2x} \\ 
    & m(m + 2) = 0 & y_p'' = 2A + 4Cxe^{-2x} - 4Ce^{-2x}\\ 
    & m = 0, -2 \\
    & y_c = c_1 + c_2e^{-2x}  \\ && 2A + 4Cxe^{-2x} - 4Ce^{-2x} + 4Ax + 2B - 4Cxe^{-2x} + 2Ce^{-2x} = 2x + 5 - e^{-2x} \\ 
    && 4Ax + 2(A+B) +2Ce^{-2x} = 2x + 5 - e^{-2x} \\
    && A =\frac{1}{2}, B = 2, C = \frac{1}{2}
\end{align*}
Our solution is:
\begin{align*}
    y_c + y_p = \Aboxed{c_1 + c_2e^{-2x} +\frac{1}{2}x^2 + 2x + \frac{1}{2}xe^{-2x}}
\end{align*}

b) $ y'' - 9y' = 2e^{3x }$
\begin{align*}
    & y'' - 9y' = 2e^{3x} && y_p = Ae^{3x}\\
    & m^2 - 9m = 0 && y_p' = 3Ae^{3x}\\
    & m(m-9) = 0 && y_p'' = 9Ae^{3x} \\
    & m = 9, 0 \\
    & y_c = c_1 + c_2e^{9x} && 9Ae^{3x} - 27Ae^{3x} = 2e^{3x} \\
    &&& -18Ae^{3x} = 2e^{3x} \\
    &&& A = -\frac{1}{9}
\end{align*}
Our solution is then:
\begin{align*}
    y_c + y_p = \Aboxed{c_1 + c_2e^{9x} - \frac{1}{9}e^{3x}}
\end{align*}
c) $ y'' + 4y' + 4y = (3+x)e^{-2x}$
\begin{align*}
    & y'' + 4y' + 4y = (3+x)e^{-2x} && y_p = Ax^2e^{-2x} + Bx^3e^{-2x}\\
    & m^2 + 4m + 4 = 0 && y_p' = 2Axe^{-2x} - 2Ax^2e^{-2x} + 3Bx^2e^{-2x} - 2Bx^3e^{-2x} \\
    & (m+2)(m+2) = 0 && y_p''= 2Ae^{-2x} + 4Ae^{-2x} - 8Ae^{-2x}\\
    & m = -2 && +4Bx^3e^{-2x} - 12Bx^2e^{-2x} + 6Bxe^{-2x} \\
    & y_c = c_1e^{-2x} + c_2xe^{-2x}
\end{align*}
Here is the nasty after plugging in:
\begin{align*}
    & 2Ae^{-2x} + 4Ae^{-2x} - 8Ae^{-2x} + 4Bx^3e^{-2x} - 12Bx^2e^{-2x} + 6Bxe^{-2x} \\
    & + 8Axe^{-2x} - 8Ax^2e^{-2x} + 12Bx^2e^{-2x} - 8Bx^3e^{-2x} \\
    & + Ax^2e^{-2x} + Bx^3e^{-2x} \\
    & = 3e^{-2x} + xe^{-2x}
\end{align*}
Simplifies beautifully into:
\begin{align*}
    & 2Ae^{-2x} + 6Bxe^{-2x} =  3e^{-2x} + xe^{-2x} \\
    & A = \frac{3}{2}, B = \frac{1}{6}
\end{align*}
Our solution is then :
\begin{align*}
    y_c + y_p = \Aboxed{c_1e^{-2x} + c_2xe^{-2x} + \frac{3}{2}x^2e^{-2x} + \frac{1}{6}x^3e^{-2x}}
\end{align*}

\setcounter{subsection}{6}
\setcounter{subsubsection}{0}
\subsubsection{}
We proceed to solve the problem $ 3y'' + y' = 9x $ using variation of parameters where our $ y_p = u_1y_1 + u_2y_2$.

\begin{align*}
    & y'' + \frac{y'}{3} = 3x  && W =  
    \begin{vmatrix}
        1 & e^{\frac{-x}{3}} \\
        0 & -\frac{1}{3}e^{\frac{-x}{3}} 
    \end{vmatrix} = -\frac{1}{3}e^{\frac{-x}{3}} 
    \\
    & m^2 + \frac{m}{3} = 0 && W_1 =
    \begin{vmatrix}
        0 & e^{\frac{-x}{3}} \\
        3x & -\frac{1}{3}e^{\frac{-x}{3}} 
    \end{vmatrix} = -3xe^{\frac{-x}{3}}  
    \\
    & m(m + \frac{1}{3}) = 0 && W_2 =
    \begin{vmatrix}
        1 & 0 \\
        0 & 3x 
    \end{vmatrix} = 3x 
    \\
    & m = 0, m = -\frac{1}{3} && u_1 = \int \frac{-3xe^{\frac{-x}{3}}}{-\frac{1}{3}e^{\frac{-x}{3}}} = \frac{9x^2}{2} \\
    & y_c = c_1 + c_2e^{\frac{-x}{3}} && u_2 = \int \frac{3x}{-\frac{1}{3} e^{\frac{-x}{3}}} = -27e^{\frac{x}{3}}(x-3)
\end{align*}
Our $y_p $ should be $u_1*1 + u_2 * e^{\frac{-x}{3}}$. We proceed to plug in for $u_1$ and $u_2$, 
I'm assuming the 81 below gets absorbed into $c_1$ since its a constant too, our answer should be: 
\begin{align*}
    y_c + y_p = c_1 + c_2e^{-\frac{x}{3}} + \frac{9x^2}{3} - 27x + 81 \\
    \Aboxed{c_1 + c_2e^{-\frac{x}{3}} + \frac{9x^2}{3} - 27x}
\end{align*}
\subsubsection{}
We solve for the initial value problem $y'' - 4y' + 4y = (6x^2 - 12x)e^{2x}$, $y(0) = 1$, $y'(0) = 0$.
Gonna skip the bits with finding our complimentary solution since the roots to $m^2 - 4m + 4$ is $ 2 $, $y_c =
c_1e^{2x} + c_2xe^{2x} $
\begin{align*}
    & y_c = c_1e^{2x} + c_2xe^{2x}
    & y_p = u_1e^{2x} + u_2xe^{2x}
\end{align*}
Now lets find $u_1$ and $u_2$:
\begin{align}
    W_1 &= 
    \begin{vmatrix}
        e^{2x} & xe^{2x} \\
        2e^{2x} & 2xe^{2x}+e^{2x} 
    \end{vmatrix} = (2xe^{4x} + e^{4x}) - 2xe^{4x} = e^{4x} \\
    W_2 &= 
    \begin{vmatrix}
        0 & xe^{2x} \\
        (6x^2-12x)e^{2x} & 2xe^{2x} + e^{2x} 
    \end{vmatrix} = -xe^{4x}(6x^2-12x) 
   \\ 
    W_3 &= 
    \begin{vmatrix}
        e^{2x} & 0 \\
        2e^{2x} & (6x^2-12x)e^{2x}  
    \end{vmatrix} = e^{4x}(6x^2 - 12x) \\
    u_1 &= \int\frac{-xe^{4x}(6x^2-12x)}{e^{4x}}dx = \int (-6x^3 + 12x^2)dx = -\frac{3}{2}x^4 + 4x^3 \\
    u_2 &= \int\frac{e^{4x}(6x^2-12x)}{e^{4x}}dx = \int(6x^2 - 12x)dx = 2x^3 - 6x^2 \\
    y_c + y_p &= c_1e^{2x} + c_2xe^{2x} + ( -\frac{3}{2}x^4 + 4x^3)e^{2x} + ( 2x^3 - 6x^2)xe^{2x} \\
    &= c_1e^{2x} + c_2xe^{2x} + \frac{1}{2}x^4e^{2x} + 2x^3e^{2x} 
\end{align}
Now that we have our general solution, its time to find its derivative, plug in our initial conditions and solve the subsequent system of equations for $c_1$ and $c_2$
\begin{align*}
    y &= c_1e^{2x} + c_2xe^{2x} + \frac{1}{2}x^4e^{2x} + 2x^3e^{2x}\\
    y'&= 2c_1e^{2x} + c_2(2xe^{2x} + e^{2x}) + \frac{1}{4}(4x^3e^{2x} + 2x^4e^{2x}) + 2(3x^2e^{2x} + 2x^3e^{2x})\\
    &y(0) = c_1 = 1 \\
    &y'(0) = 2 + c_2 =  0,  c_2 = -2 \\
\end{align*}
Turned out not to have been much of a system since plugging in gave us the solution thankfully(or I might be a complete idiot). Our solution is:
\begin{align*}
    \Aboxed{y = e^{2x} -2xe^{2x} + \frac{1}{2}x^4e^{2x} + 2x^3e^{2x}}
\end{align*}

\setcounter{subsection}{7}
\setcounter{subsubsection}{0}
\subsubsection{}
We are tasked with solving the following differential equations: \\
a) $4x^2y'' + y= 0$
\begin{align*}
    &  y = x^m  && 4m^2x^m-4mx^m+x^m = 0\\
    & y' = mx^{m-1} && (4m^2 -4m + 1)x^m = 0\\
    & y'' = m(m-1)x^{m-2} && (2m - 1)^2 = 0 \\
    & && m = \frac{1}{2}
\end{align*}
Simple enough, we end up with the solution:
\begin{align*}
    y = \Aboxed{c_1\sqrt{x}+c_2\sqrt{x}\ln{x}}
\end{align*}
b) $ x^2y'' - 7xy' + 41y = 0$
\begin{align*}
    &  y = x^m  && m^2x^m -8mx^m + 41x^m = 0\\
    & y' = mx^{m-1} && (m^2 - 8m + 41)x^m = 0\\
    & y'' = m(m-1)x^{m-2} && m^2 - 8m + 41 = 0
\end{align*}
We're gonna throw that quadratic into a calculator because I'm out of time, we get our roots and then our solution:
\begin{align*}
    4+5i && 4-5i\\
\end{align*}
Our answer is then:
\begin{align*}
    y = \Aboxed{c_1x^4\cos(5\ln(x)) + c_2x^4\sin(5\ln(x))}
\end{align*}
\end{document}
