\documentclass{article}
\usepackage{xcolor}
\usepackage{parskip}
\usepackage{amsmath}
\usepackage{amsthm}
\usepackage{amssymb}
\usepackage{mathtools}
\usepackage{fancyhdr}
\usepackage[%paperheight = 59.4cm,
            %paperwidth = 42cm,
            includehead,
            nomarginpar,
            textwidth=15cm,
            headheight=10mm]{geometry}


\begin{document}

\pagestyle{fancy}
%\fancyhead{}\fancyfoot{}

\fancyhf[OHC]{Christopher Munoz WRH3 Diffeq}
\setcounter{section}{2}
\setcounter{subsection}{3}
\setcounter{subsubsection}{0}
%\section{section1}

\subsection{Exact equations}
\subsubsection{problem a)}
Consider the differential equation: $(\sin(y) - y\sin(x))dx + (\cos(x) + x\cos(y) - 3y)dy = 0$, we solve via the method of exact equations:
\begin{align*}
    & M(x,y) = (\sin(y) - y\sin(x)) & \frac{\delta M}{\delta y} = \cos(y) - \sin(x)\\
    & N(x,y) = (\cos(x) + x\cos(y) - 3y) & \frac{\delta N}{\delta y} = \cos(y) - \sin(x)
\end{align*}
Now we solve:
\begin{align}
    & f(x,y) = \int(\sin(y) - y\sin(x))dx & = x\sin(y) + y\cos(x) + g(y)\\
     &\frac{\delta f}{\delta y} = \textcolor{red}{x\cos(y)} + \textcolor{red}{\cos(x)} + g'(y) =
     \textcolor{red}{\cos(x)} + \textcolor{red}{x\cos(y)} - 3y & \rightarrow  g'(y) = -3y\\
     & \int g'(y)dy = \int -3ydy\\
     & g(y) = -\frac{3}{2}y^2
\end{align}
Thus our solution is:
\begin{align}
     \Aboxed{x\sin(y) + y\cos(x) - \frac{3}{2}y^2 = C}
\end{align}



\setcounter{subsubsection}{0}\subsubsection{problem b)}
We are given the differential equation $ (y\ln(y) + e^{xy})dx + (\frac{1}{y} + x\ln(y))dy = 0 $ first we determine if it is exact: 

\setcounter{equation}{0}
\begin{align*}
    &M(x,y) = y\ln(y) + e^{xy} & \frac{\delta M}{\delta y} = \ln(y) + 1 + xe^{xy}\\
    &N(x,y) = \frac{1}{y} + x\ln(y) & \frac{\delta N}{\delta y} = \ln(y)
\end{align*}
Thus we can conclude:
\begin{align*}
    \Aboxed{\text{The Equation is not exact}}
\end{align*}\setcounter{equation}{0}

\setcounter{subsection}{3}
\subsection{problem 2}
We are given the equation $y(x + y + 1)dx + (x + 2y)dy = 0$, we first determine if it is exact or not.
\setcounter{subsubsection}{1}
%\subsection{problem 2)}
\subsubsection{a)}
\begin{align*}
    &M(x,y) = y(x + y + 1) = yx + y^2 + y & \frac{\delta M}{\delta y} = x + 2y + 1\\
    &N(x,y) = x + 2y & \frac{\delta N}{\delta y} = 1 
\end{align*}
\begin{align*}
    \frac{\delta M}{\delta y} \not= \frac{\delta N}{\delta y}\\ \Aboxed{\text{Not Exact}}
\end{align*}


\setcounter{subsubsection}{1}
For this part we add $\mu(x) = e^x$ as our integrating factor to get the equation 
$(yxe^x + y^2e^x + ye^x)dx + (xe^x + eye^x)dy = 0$:
\subsubsection{b)} 
\begin{align*}
    &M(x,y) =  yxe^x + y^2e^x + ye^x & \frac{\delta M}{\delta y} = xe^x + 2ye^x + e^x\\
    &N(x,y) = xe^x + 2ye^x & \frac{\delta N}{\delta y} = e^x + xe^x + 2ye^x
\end{align*}
\begin{align*}
    \frac{\delta M}{\delta y} = \frac{\delta N}{\delta y}\\ \Aboxed{\text{Exact Equation}}
\end{align*}

\setcounter{subsubsection}{1}
Now we find the solution:
\subsubsection{c)} 
\begin{align}
    & f(x,y) = \int(yxe^x + y^2e^x + ye^x) &= e^xy^2 + e^xy + g(y) \\
    & \frac{\delta f}{\delta y} = \textcolor{red}{2e^xy+xe^x = xe^x + 2ye^x} & g(y) = 0
\end{align}
\begin{align}
     \Aboxed{e^xy^2 + e^xxy = C}
\end{align}

\end{document}
