\documentclass{article}
\usepackage{xcolor}
\usepackage{tikz}
\usepackage{parskip}
\usepackage{amsmath}
\usepackage{amsthm}
\usepackage{amssymb}
\usepackage{mathtools}
\usepackage{fancyhdr}
\usepackage[%paperheight = 59.4cm,
            %paperwidth = 42cm,
            %includehead,
            nomarginpar,
            textwidth=15cm,
            headheight=10mm]{geometry}


\begin{document}

\pagestyle{fancy}
%\fancyhead{}\fancyfoot{}

\fancyhf[OHC]{Christopher Munoz WRH5 Diffeq}
\setcounter{section}{4}
\setcounter{subsection}{2}
\setcounter{subsubsection}{0}
\subsubsection{} 
 We are given the differential equation $ y'' + 2y' + y = 0$ with the solution $y_1 = xe^{-x}$ we will construct the second solution using the formula provided: $y_2 = y_1\int \frac{e^{- \int p(x)dx}}{(y_1)^2}dx$.
\begin{align}
    y_2 &= y_1\int \frac{e^{- \int p(x)dx}}{(y_1)^2}dx \\ 
    &  = xe^{-x}\int \frac{e^{- \int 2dx}}{(xe^{-x})^2}dx & p(x) = 2  \\
    & = xe^{-x}\int \frac{e^{-2x}}{(xe^{-x})^2}dx \\
    & = xe^{-x}\int \frac{e^{-2x}}{(x^2e^{-2x})}dx \\
    & = xe^{-x}\int \frac{1}{x^2}dx \\
    & = xe^{-x} \int (\frac{\sec(\ln(x))}{x}) \\
    & = -e^{-x}
\end{align}
Our second solution is 
\begin{align*}
    \Aboxed{y_2 = C_2 e^{-x}}
\end{align*}
\subsubsection{} 
We are given the differential equation $x^2y'' - 3xy' + 5y = 0$ with the solution $y_1 = x^2 \cos(\ln(x))$ we will construct the second solution using the formula provided: $y_2 = y_1\int \frac{e^{- \int p(x)dx}}{(y_1)^2}dx$.

First we divide our equation $x^2y'' - 3xy' + 5y = 0$ by its leading term $x^2$:  
\setcounter{equation}{0}
\begin{align*}
    \frac{x^2y'' - 3xy' + 5y}{x^2} = y'' - \frac{3y'}{x} + \frac{5y}{x^2}
\end{align*}
Our $p (x) $ term is now $-\frac{3}{x}$, now we just plug in and solve:
\begin{align}
    y_2 &= y_1\int \frac{e^{- \int p(x)dx}}{(y_1)^2}dx \\ 
    &  = x^2 \cos(\ln(x)) \int \frac{e^{- \int -\frac{3}{x}dx}}{(x^2 \cos(\ln(x)))^2}dx & p(x) = - \frac{3}{x}  \\
    & = x^2 \cos(\ln(x)) \int \frac{e^{3\ln(x)}}{(x^2 \cos(\ln(x)))^2}dx \\
    & = x^2 \cos(\ln(x)) \int \frac{x^3}{(x^4 \cos^2(\ln(x)))}dx \\
    & = x^2 \cos(\ln(x)) \int \frac{1}{xcos^2(\ln(x))}dx \\
    & = x^2 \cos(\ln(x)) \int \frac{\sec^2(\ln(x))}{x} \\
    & = x^2 \cos(\ln(x)) \int {\sec^2(u)}du & u = \ln(x) && du = \frac{1}{x}\\
    & = x^2 \cos(\ln(x)) * \tan(\ln(x))\\
    & = x^2 \cos(\ln(x)) * \frac{\sin(\ln(x))}{\cos(\ln(x))} \\
    & = x^2 \sin(\ln(x))
\end{align}
Thus our second solution is:
\begin{align*}
    \Aboxed{y_2 = C_2x^2 \sin(\ln(x))}
\end{align*}
\subsubsection{} \setcounter{equation}{0}
We are given the differential equation $y'' + 16y = 0$ with the solution of $y_1 = \sin(4x)$. We will find the second solution using the reduction of order technique assuming $y_2 = uy_1$, first some derivatives
\begin{align*}
    y_2 &= uy_1 && y_1 = \sin(4x)\\
    y_2' &= u'y_1 + uy_1'' && y_1' = 4\cos(4x) \\
    y_2'' &= u''y_1 + 2u'y_1' + uy_1''&& y_1'' = -16\sin(4x)
\end{align*}
Next we plug in our derivatives into the original equation:
\begin{align}
    u''y_1 + 2u'y_1' + uy_1'' + 16(uy_1) = 0
\end{align}
and our y's, simplify and solve:
\begin{align}
     u''\sin(4x) + 8u'\cos(4x)-16u\sin(4x) + 16u\sin(4x) = 0\\
     u''\sin(4x) + 8u'\cos(4x)+16u(\sin(4x) - \sin(4x)) = 0\\
     u''\sin(4x) + 8u'\cos(4x) = 0 && w' = u'', w = u'\\
     w'\sin(4x) + 8w\cos(4x) = 0 \\
     w' + 8w\cot(4x) = 0 \\
\end{align}
Got stuck
\subsection{}
\subsubsection{}
The following is mostly factoring and algebra:
\newline a) $20y'' - y' - y = 0$
\begin{align*}
    20m^2 - m - 1 = 0 \\
    (4m-1)(5m+1) = 0 && m = \frac{1}{4}, -\frac{1}{5} \\
    \Aboxed{y = c_1e^{\frac{-x}{5}} + c_2e^{\frac{x}{4}}}
\end{align*}
b) $ y'' - 10y' + 25y = 0$
\begin{align*}
    m^2 - 10m + 25 = 0 \\
    (m-5)(m-5) = 0 && m = 5 \\
    \Aboxed{y = c_1e^{5x} + c_2xe^{5x}}
\end{align*}
c) $ 5y'' + y = 0$
\begin{align*}
    5m^2 + 1 = 0 \\
    m^2 = -\frac{1}{5} && m = \frac{i}{\sqrt{5}}, -\frac{i}{\sqrt{5}} \\
    \Aboxed{y = c_1\cos(\frac{x}{\sqrt{5}}) + c_2\sin(\frac{x}{\sqrt{5}})}
\end{align*}
d) $ y^{(4)} - 2y'' + y = 0$
\begin{align*}
    m^4 -2m^2 + 1 = 0\\
    (m+1)^2(m-1)^2 && m = 1,-1 \\
    \Aboxed{y = c_1e^{-x} + c_2xe^{-x} + c_3e^x + c_4xe^x}
\end{align*}
e) $ y^{(5)} + y^{(4)} - y''' = 0$
\begin{align*}
    m^5 + m^4 - m^3 = 0\\
    m^3(m^2+m-1) && \text{Use quadratic formula for right side} \\ 
    m = 0,\frac{\sqrt{5}-1}{2},\frac{-\sqrt{5}-1}{2} \\
    \Aboxed{y = c_1+c_2e^{\frac{x\sqrt{5}-1}{2}} + c_3e^{\frac{-x\sqrt{5}-1}{2}}}
\end{align*}
I hope that's the answer
\subsubsection{}
We can find a differential equation whos solution is $c_1e^{9x} + c_2xe^{9x}$ by finding a quadratic equation whos root is 9 and 9 alone, so I'm going to go ahead and steal problem be from 4.3.1.
\begin{align*}
    (m-9)(m-9) \\
    m^2 - 18m + 81 = 0 \\
    \Aboxed{ y'' - 18y' +81y = 0}
\end{align*}
\subsubsection{}
Here we solve the initial value problem $y'' + 2y' + y = 0$ with $y(0) = 5$ and $y'(0) = 10$
\begin{align*}
    m^2 + 2m + 1 = 0 \\
    (m+1)(m+1) = 0 && m = -1\\
    y = c_1e^{-x} + c_2xe^{-x}
\end{align*}
now for our actual solution:
\begin{align*}
    y &= c_1e^{-x} + c_2xe^{-x} \\
    y'&= -c_1e^{-x} + c_2(e^{-x} - xe^{-x}) && 10 = c_2 \\
    & \Aboxed{y = 5e^{-x} + 10xe^{-x}}
\end{align*}
Ran out of time for the rest




\end{document}
